feat: symbol exec

qcp/ast/annotated_C/alpha_equiv.c
@@ -1,7 +1,21 @@
 #include "ast.h"
 
-bool alpha_equiv(term *t1, term *t2) {
+bool alpha_equiv(term *t1, term *t2)
+/*@ With term1 term2
+      Require store_term(t1, term1) *
+              store_term(t2, term2)
+      Ensure __return == term_eqn(term1, term2) && t1 == t1@pre && t2 == t2@pre
+   && store_term(t1, term1) * store_term(t2, term2)
+*/
+{
   if (t1 == (void *)0 || t2 == (void *)0) return false;
+  /*@ store_term(t1, term1) * store_term(t2, term2)
+      which implies
+      data_at(&(t1 -> type), termtypeID(term1)) *
+      data_at(&(t2 -> type), termtypeID(term2)) *
+      store_term'(t1, term1) *
+      store_term'(t2, term2)
+  */
   if (t1->type != t2->type) return false;
   switch (t1->type) {
     case Var: {
