qcp/ast/annotated_C/ast.h
@@ -1,3 +1,32 @@
+/*@ Import Coq Require Import ast_lib */
+
+/*@ Extern Coq (term :: *) */
+/*@ Extern Coq (var_sub :: *) */
+/*@ Extern Coq (solve_res :: *) */
+/*@ Extern Coq (ImplyProp :: *) */
+/*@ Extern Coq (store_string : Z -> list Z -> Assertion)
+               (store_term : Z -> term -> Assertion)
+               (store_term' : Z -> term -> Assertion)
+               (store_term_cell : Z -> term -> Assertion)
+               (sll_term_list : Z -> list term -> Assertion)
+               (sllseg_term_list : Z -> list term -> Assertion)
+               (sllbseg_term_list : Z -> list term -> Assertion)
+               (store_var_sub : Z -> var_sub -> Assertion)
+               (store_var_sub_cell : Z -> var_sub -> Assertion)
+               (sll_var_sub_list : Z -> list var_sub -> Assertion)
+               (sllseg_var_sub_list : Z -> list var_sub -> Assertion)
+               (sllbseg_var_sub_list : Z -> list var_sub -> Assertion)
+               (store_solve_res : Z -> solve_res -> Assertion)
+               (store_solve_res' : Z -> solve_res -> Assertion)
+               (store_ImplyProp : Z -> Z -> Z -> term -> term -> Assertion)
+               (list_Z_cmp : list Z -> list Z -> Z)
+               (term_eqn : term -> term -> Z)
+               (term_subst_v : list Z -> list Z -> term -> term)
+               (term_subst_t : term -> list Z -> term -> term)
+               (termtypeID : term -> Z)
+*/
+
+
 typedef enum { false, true } bool;
 
 enum const_type {
@@ -75,25 +104,98 @@ typedef struct {
 /* BEGIN Given Functions */
 
 // malloc 函数，内存均初始为全0
-term_list *malloc_term_list();
-solve_res *malloc_solve_res();
+term_list *malloc_term_list()
+    /*@ Require emp
+        Ensure __return != 0 &&
+              data_at(&(__return -> element), 0) *
+              data_at(&(__return -> next), 0)
+    */
+    ;
+
+solve_res *malloc_solve_res()
+    /*@ Require emp
+        Ensure __return != 0 &&
+              data_at(&(__return -> type), 0) *
+              data_at(&(__return -> d), 0)
+    */
+    ;
 
 // 构造函数
-ImplyProp *createImplyProp(term *t1, term *t2);
+ImplyProp *createImplyProp(term *t1, term *t2)
+    /*@ With term1 term2
+          Require store_term(t1, term1) *
+                  store_term(t2, term2)
+          Ensure t1 == t1@pre && t2 == t2@pre &&
+                store_ImplyProp(__return, t1, t2, term1, term2)
+    */
+    ;
 
 // 深拷贝函数
-term *copy_term(term *t);
-term_list *copy_term_list(term_list *list);
+term *copy_term(term *t)
+    /*@ With _term
+          Require store_term(t, _term)
+          Ensure __return != 0 &&
+                store_term(t, _term) *
+                store_term(__return, _term)
+    */
+    ;
+
+term_list *copy_term_list(term_list *list)
+    /*@ With l
+          Require sll_term_list(list, l)
+          Ensure __return != 0 &&
+                sll_term_list(list, l) *
+                sll_term_list(__return, l)
+    */
+    ;
 
 // free 函数
-void free_str(char *s);
-void free_imply_prop(ImplyProp *p);
-void free_term(term *t);
-void free_term_list(term_list *list);
+void free_str(char *s)
+    /*@ Require s != 0 && exists n, n > 0 && store_undef_char_array(s, n)
+        Ensure emp
+    */
+    ;
+
+void free_imply_prop(ImplyProp *p)
+    /*@ With term1 term2 t1 t2
+          Require store_ImplyProp(p, t1, t2, term1, term2)
+          Ensure store_term(t1, term1) *
+                store_term(t2, term2) *
+                emp
+    */
+    ;
+
+void free_term(term *t)
+    /*@ Require exists _term, store_term(t, _term)
+        Ensure emp
+    */
+    ;
+
+void free_term_list(term_list *list)
+    /*@ Require exists l, sll_term_list(list, l)
+        Ensure emp
+    */
+    ;
 
 // string 相关函数
-char *strdup(const char *s);
-int strcmp(const char *s1, const char *s2);
+char *strdup(const char *s)
+    /*@ With n str
+          Require store_char_array(s, n, str)
+          Ensure __return != 0 &&
+                store_char_array(s, n, str) *
+                store_char_array(__return, n, str)
+    */
+    ;
+
+int strcmp(const char *s1, const char *s2)
+    /*@ With str1 str2 n1 n2
+          Require store_char_array(s1, n1, str1) *
+                  store_char_array(s2, n2, str2)
+          Ensure __return == list_Z_cmp(str1, str2) &&
+                store_char_array(s1, n1, str1) *
+                store_char_array(s2, n2, str2)
+    */
+    ;
 
 /* END Given Functions */
 
