qcp/ast/annotated_C/subst.c
@@ -1,6 +1,16 @@
 #include "ast.h"
 
-term* subst_var(char* den, char* src, term* t) {
+term *subst_var(char *den, char *src, term *t)
+/*@ With term src_str den_str
+      Require store_term(t, term) *
+              store_string(src, src_str) *
+              store_string(den, den_str)
+      Ensure __return == t && t == t@pre && den == den@pre && src == src@pre &&
+             store_term(t, term_subst_v(den, src, term)) *
+             store_string(den, den_str) *
+             store_string(src, src_str)
+*/
+{
   switch (t->type) {
     case Var: {
       if (!strcmp(t->content.Var, src)) {
@@ -30,7 +40,16 @@ term* subst_var(char* den, char* src, term* t) {
   return t;
 }
 
-term* subst_term(term* den, char* src, term* t) {
+term *subst_term(term *den, char *src, term *t)
+/*@ With term src_str den_term
+      Require store_term(t, term) *
+              store_string(src, src_str) *
+              store_term(den, den_term)
+      Ensure __return == t && t == t@pre && den == den@pre && src == src@pre &&
+             store_term(t, term_subst_t(den, src, term)) *
+             store_term(den, den_term) *
+             store_string(src, src_str)
+*/{
   switch (t->type) {
     case Var: {
       if (!strcmp(t->content.Var, src)) {
