qcp/ast/lib/ast_lib.v
@@ -17,12 +17,12 @@ Local Open Scope list.
 Require Import String.
 Local Open Scope string.
 From SimpleC.EE Require Import sll_tmpl.
+From SimpleC.EE Require Import malloc.
 
 Import naive_C_Rules.
 Local Open Scope sac.
 
 Definition var_name : Type := list Z.
-
 
 (* all about ast basic structure *)
 Module ast_def.
@@ -96,15 +96,6 @@ Definition termtypeID (t: term) : Z :=
 (* Definition zlength {A: Type} (l: list A) : Z :=
   Z.of_nat (List.length l). *)
 
-Fixpoint all_zero_list_nat (n: nat) : list Z :=
-  match n with
-    | O => nil
-    | S n0 => 0 :: (all_zero_list_nat n0)
-  end.
-
-Definition all_zero_list (n: Z): list Z :=
-  all_zero_list_nat (Z.to_nat n).
-
 Definition store_string (x: addr) (str: var_name): Assertion :=
   EX n: Z,
   [| n >= 0 |] &&
@@ -127,6 +118,112 @@ Fixpoint store_term (x: addr) (t: term): Assertion :=
                                   &(x # "term" ->ₛ "content" .ₛ "Quant" .ₛ "body") # Ptr |-> z **
                                   store_string y qvar ** store_term z body
   end.
+
+Definition store_term' (x: addr) (t: term): Assertion :=
+  match t with
+    | TermVar var => [| x <> NULL |] &&
+                     EX y: addr,
+                      &(x # "term" ->ₛ "content" .ₛ "Var") # Ptr |-> y **
+                      store_string y var
+    | TermConst ctype content => [| x <> NULL |] &&
+                                 &(x # "term" ->ₛ "content" .ₛ "Const" .ₛ "type") # Int |-> ctID ctype **
+                                 &(x # "term" ->ₛ "content" .ₛ "Const" .ₛ "content") # Int |-> content
+    | TermApply lt rt => [| x <> NULL |] && 
+                         EX y z: addr,
+                          &(x # "term" ->ₛ "content" .ₛ "Apply" .ₛ "left") # Ptr |-> y **
+                          &(x # "term" ->ₛ "content" .ₛ "Apply" .ₛ "right") # Ptr |-> z **
+                          store_term y lt ** store_term z rt
+    | TermQuant qtype qvar body => [| x <> NULL |] && 
+                                   EX y z: addr,
+                                    &(x # "term" ->ₛ "content" .ₛ "Quant" .ₛ "var") # Ptr |-> y **
+                                    &(x # "term" ->ₛ "content" .ₛ "Quant" .ₛ "body") # Ptr |-> z **
+                                    store_string y qvar ** store_term z body
+  end.
+
+Lemma store_term_unfold: forall x t,
+  store_term x t |--
+  &(x # "term" ->ₛ "type") # Int |-> termtypeID t **
+  store_term' x t.
+Proof.
+  intros.
+  unfold store_term, store_term'.
+  destruct t; fold store_term; entailer!.
+Qed.
+
+Lemma store_term_fold: forall x t,
+  &(x # "term" ->ₛ "type") # Int |-> termtypeID t **
+  store_term' x t |--
+  store_term x t.
+Proof.
+  intros.
+  unfold store_term, store_term'.
+  destruct t; fold store_term; entailer!.
+Qed.
+
+Lemma store_term'_Var: forall x t,
+  termtypeID t = 0%Z ->
+  store_term' x t |--
+  EX var, [| t = TermVar var |] && [| x <> NULL |] &&
+  EX y: addr,
+    &(x # "term" ->ₛ "content" .ₛ "Var") # Ptr |-> y **
+    store_string y var.
+Proof.
+  intros.
+  unfold store_term'.
+  induction t; try discriminate.
+  Intros y.
+  Exists var y.
+  entailer!.
+Qed.
+
+Lemma store_term'_Const: forall x t,
+  termtypeID t = 1%Z ->
+  store_term' x t |--
+  EX ctype content, [| t = TermConst ctype content |] && [| x <> NULL |] &&
+  &(x # "term" ->ₛ "content" .ₛ "Const" .ₛ "type") # Int |-> ctID ctype **
+  &(x # "term" ->ₛ "content" .ₛ "Const" .ₛ "content") # Int |-> content.
+Proof.
+  intros.
+  unfold store_term'.
+  induction t; try discriminate.
+  Intros.
+  Exists ctype content.
+  entailer!.
+Qed.
+
+Lemma store_term'_Apply: forall x t,
+  termtypeID t = 2%Z ->
+  store_term' x t |--
+  EX lt rt, [| t = TermApply lt rt |] && [| x <> NULL |] &&
+  EX y z: addr,
+    &(x # "term" ->ₛ "content" .ₛ "Apply" .ₛ "left") # Ptr |-> y **
+    &(x # "term" ->ₛ "content" .ₛ "Apply" .ₛ "right") # Ptr |-> z **
+    store_term y lt ** store_term z rt.
+Proof.
+  intros.
+  unfold store_term'.
+  induction t; try discriminate.
+  Intros y z.
+  Exists t1 t2 y z.
+  entailer!.
+Qed.
+
+Lemma store_term'_Quant: forall x t,
+  termtypeID t = 3%Z ->
+  store_term' x t |--
+  EX qtype qvar body, [| t = TermQuant qtype qvar body |] && [| x <> NULL |] &&
+  EX y z: addr,
+    &(x # "term" ->ₛ "content" .ₛ "Quant" .ₛ "var") # Ptr |-> y **
+    &(x # "term" ->ₛ "content" .ₛ "Quant" .ₛ "body") # Ptr |-> z **
+    store_string y qvar ** store_term z body.
+Proof.
+  intros.
+  unfold store_term'.
+  induction t; try discriminate.
+  Intros y z.
+  Exists qtype qvar t y z.
+  entailer!.
+Qed.
 
 Definition store_term_cell (x: addr) (t: term): Assertion :=
   [| x <> NULL |] &&
@@ -216,6 +313,64 @@ Definition store_solve_res (x: addr) (sr: solve_res): Assertion :=
                    sll_term_list y l
   end.
 
+Definition store_solve_res' (x: addr) (sr: solve_res): Assertion :=
+  match sr with
+    | SRBool ans => [| x <> NULL |] && &(x # "solve_res" ->ₛ "content" .ₛ "Bool") # Int |-> ans
+    | SRTList l => [| x <> NULL |] && EX y: addr,
+                   &(x # "solve_res" ->ₛ "content" .ₛ "TermList") # Ptr |-> y **
+                   sll_term_list y l
+  end.
+
+Lemma store_solve_res_unfold: forall x sr,
+  store_solve_res x sr |--
+  &(x # "solve_res" ->ₛ "type") # Int |-> restypeID sr **
+  store_solve_res' x sr.
+Proof.
+  intros.
+  unfold store_solve_res, store_solve_res'.
+  destruct sr; fold store_solve_res; entailer!.
+Qed.
+
+Lemma store_solve_res_fold: forall x sr,
+  &(x # "solve_res" ->ₛ "type") # Int |-> restypeID sr **
+  store_solve_res' x sr |--
+  store_solve_res x sr.
+Proof.
+  intros.
+  unfold store_solve_res, store_solve_res'.
+  destruct sr; fold store_solve_res; entailer!.
+Qed.
+
+Lemma store_solve_res'_Bool: forall x sr,
+  restypeID sr = 0%Z ->
+  store_solve_res' x sr |--
+  EX ans, [| sr = SRBool ans |] && [| x <> NULL |] &&
+  &(x # "solve_res" ->ₛ "content" .ₛ "Bool") # Int |-> ans.
+Proof.
+  intros.
+  unfold store_solve_res'.
+  induction sr; try discriminate.
+  Intros.
+  Exists ans.
+  entailer!.
+Qed.
+
+Lemma store_solve_res'_List: forall x sr,
+  restypeID sr = 1%Z ->
+  store_solve_res' x sr |--
+  EX l, [| sr = SRTList l |] && [| x <> NULL |] &&
+  EX y: addr,
+    &(x # "solve_res" ->ₛ "content" .ₛ "TermList") # Ptr |-> y **
+    sll_term_list y l.
+Proof.
+  intros.
+  unfold store_solve_res'.
+  induction sr; try discriminate.
+  Intros y.
+  Exists l y.
+  entailer!.
+Qed.
+
 (* all about ImplyProp *)
 
 Module ast_imply_prop.
@@ -223,15 +378,63 @@ Module ast_imply_prop.
 Inductive ImplyProp : Type :=
   | ImplP (assum: term) (concl: term): ImplyProp.
 
-Definition store_ImplyProp (x: addr) (p: ImplyProp): Assertion :=
-  match p with
-    | ImplP assum concl => [| x <> NULL |] &&
-                           EX y z: addr,
-                            &(x # "ImplyProp" ->ₛ "assum") # Ptr |-> y **
-                            &(x # "ImplyProp" ->ₛ "concl") # Ptr |-> z **
-                            store_term y assum ** store_term z concl
-  end.
+Definition store_ImplyProp (x y z: addr) (assum concl: term): Assertion :=
+  [| x <> NULL |] &&
+  &(x # "ImplyProp" ->ₛ "assum") # Ptr |-> y **
+  &(x # "ImplyProp" ->ₛ "concl") # Ptr |-> z **
+  store_term y assum ** store_term z concl.
 
 End ast_imply_prop.
 
 Import ast_imply_prop.
+
+Fixpoint list_Z_eqb (l1 l2 : list Z) : bool :=
+  match l1, l2 with
+  | [], [] => true
+  | x1 :: t1, x2 :: t2 => Z.eqb x1 x2 && list_Z_eqb t1 t2
+  | _, _ => false
+  end.
+
+Definition list_Z_cmp (l1 l2 : list Z) : Z :=
+  if list_Z_eqb l1 l2 then 0 else 1.
+
+Fixpoint term_eqb (t1 t2: term): bool :=
+  match t1, t2 with
+    | TermVar v1, TermVar v2 => list_Z_eqb v1 v2
+    | TermConst ctype1 content1, TermConst ctype2 content2 =>
+      (Z.eqb (ctID ctype1) (ctID ctype2)) && (Z.eqb content1 content2)
+    | TermApply lt1 rt1, TermApply lt2 rt2 =>
+      term_eqb lt1 lt2 && term_eqb rt1 rt2
+    | TermQuant qtype1 qvar1 body1, TermQuant qtype2 qvar2 body2 =>
+      (Z.eqb (qtID qtype1) (qtID qtype2)) &&
+      list_Z_eqb qvar1 qvar2 &&
+      term_eqb body1 body2
+    | _, _ => false
+  end.
+
+Definition term_eqn (t1 t2: term): Z :=
+  if term_eqb t1 t2 then 1 else 0.
+
+Fixpoint term_subst_v (den src: var_name) (t: term): term :=
+  match t with
+    | TermVar v => if list_Z_eqb v src then TermVar den else TermVar v
+    | TermConst ctype content => TermConst ctype content
+    | TermApply lt rt => TermApply (term_subst_v den src lt) (term_subst_v den src rt)
+    | TermQuant qtype qvar body =>
+      if list_Z_eqb qvar src then
+        TermQuant qtype qvar body
+      else
+        TermQuant qtype qvar (term_subst_v den src body)
+  end.
+
+Fixpoint term_subst_t (den: term) (src: var_name) (t: term): term :=
+  match t with
+    | TermVar v => if list_Z_eqb v src then den else TermVar v
+    | TermConst ctype content => TermConst ctype content
+    | TermApply lt rt => TermApply (term_subst_t den src lt) (term_subst_t den src rt)
+    | TermQuant qtype qvar body =>
+      if list_Z_eqb qvar src then
+        TermQuant qtype qvar body
+      else
+        TermQuant qtype qvar (term_subst_t den src body)
+  end.
