qcp/cnf/lib/cnf_trans_lib.v
@@ -21,47 +21,31 @@ Import naive_C_Rules.
 Local Open Scope sac.
 
 From SimpleC.EE Require Import sll_tmpl.
+From SimpleC.EE Require Import malloc.
+From SimpleC.EE Require Import smt_lang_lib.
 
-Inductive cnf_list_cell : Type :=
-  | CNFCell (size: Z) (clause: list Z): cnf_list_cell.
+Definition cnf_list_cell := list Z.
 
-Definition cnf_list : Type := list cnf_list_cell.
+Definition cnf_list : Type := list (list Z).
 
-Inductive PreData : Type :=
-  | PD (cnf_res: cnf_list) (prop_cnt: Z) (clause_cnt: Z): PreData.
+(* Inductive PreData : Type :=
+  | PD (cnf_res: cnf_list) (prop_cnt: Z) (clause_cnt: Z): PreData. *)
 
 (* Print store_int_array. *)
+Definition init_int_array (x: addr) (size: Z): Assertion :=
+  store_int_array x size (all_zero_list size).
 
-Definition store_cnf_list_cell (x: addr) (c: cnf_list_cell): Assertion :=
-  match c with
-    | CNFCell size clause => [| x <> NULL |] && [| Zlength clause = size |] &&
-                             EX y: addr,
-                              &(x # "cnf_list" ->ₛ "size") # Int |-> size **
-                              &(x # "cnf_list" ->ₛ "clause") # Ptr |-> y **
-                              store_int_array y size clause
-  end.
+Definition store_clause (x: addr) (clause: list Z): Assertion :=
+ [| Zlength clause <= 3 |] && [| Forall (fun z => z <> 0) clause |] &&
+  store_int_array x 3%Z (clause ++ all_zero_list (3 - Zlength clause)).
 
-(* Definition link_cnf_list_cell (x y: addr): Assertion :=
-  [| x <> NULL |] &&
-  &(x # "cnf_list" ->ₛ "next") # Ptr |-> y. *)
+Definition store_cnf_list_cell (x: addr) (clause: list Z): Assertion :=
+ [| x <> NULL |] && EX y: addr,
+  &(x # "cnf_list" ->ₛ "size") # Int |-> 3%Z **
+  &(x # "cnf_list" ->ₛ "clause") # Ptr |-> y **
+  store_clause y clause.
 
-Module cnf_list_store_lists1.
-
-Fixpoint sll_cnf_list (x: addr) (l: cnf_list): Assertion :=
-  match l with
-    | nil => [| x = NULL |] && emp
-    | (CNFCell size clause) :: l0 => [| x <> NULL |] && [| Zlength clause = size |] &&
-                                   EX y z: addr,
-                                    &(x # "cnf_list" ->ₛ "size") # Int |-> size **
-                                    &(x # "cnf_list" ->ₛ "clause") # Ptr |-> y **
-                                    &(x # "cnf_list" ->ₛ "next") # Ptr |-> z **
-                                    store_int_array y size clause **
-                                    sll_cnf_list z l0
-  end.
-
-End cnf_list_store_lists1.
-
-Module cnf_list_store_lists2.
+Module cnf_list_store_lists.
 
 Definition sll_cnf_list (x: addr) (l: cnf_list): Assertion :=
   sll store_cnf_list_cell "cnf_list" "next" x l.
@@ -72,16 +56,12 @@ Definition sllseg_cnf_list (x: addr) (y: addr) (l: cnf_list): Assertion :=
 Definition sllbseg_cnf_list (x: addr) (y: addr) (l: cnf_list): Assertion :=
   sllbseg store_cnf_list_cell "cnf_list" "next" x y l.
 
-End cnf_list_store_lists2.
+End cnf_list_store_lists.
 
-Import cnf_list_store_lists2.
+Import cnf_list_store_lists.
 
-(* Definition zlength {A: Type} (l: list A) : Z :=
-  Z.of_nat (List.length l). *)
-
-Definition Z_union (l1 l2 : list Z) : list Z :=
+(* Definition Z_union (l1 l2 : list Z) : list Z :=
   nodup Z.eq_dec (l1 ++ l2).
-
 
 Fixpoint all_vars (l: cnf_list): list Z :=
   match l with
@@ -90,17 +70,308 @@ Fixpoint all_vars (l: cnf_list): list Z :=
   end.
 
 Definition all_vars_cnt (l: cnf_list): Z :=
-  Zlength (all_vars l).
+  Zlength (all_vars l). *)
 
-(* Compute Z_union [1; 2; 3] [2; 4; 5; 1]. *)
-  (* = [1; 2; 3; 4; 5] : list Z *)
+Fixpoint max_element (l: list Z): Z :=
+  match l with
+    | nil => 0%Z
+    | h :: t => Z.max h (max_element t)
+  end.
 
-Definition store_predata (x: addr) (p: PreData): Assertion :=
-  match p with
-    | PD cnf_res prop_cnt clause_cnt => [| x <> NULL |] && [| Zlength cnf_res = clause_cnt |] && [| all_vars_cnt cnf_res = prop_cnt |] &&
-                                        EX y: addr,
-                                         &(x # "PreData" ->ₛ "cnf_res") # Ptr |-> y **
-                                         &(x # "PreData" ->ₛ "prop_cnt") # Int |-> prop_cnt **
-                                         &(x # "PreData" ->ₛ "clause_cnt") # Int |-> clause_cnt **
-                                         sll_cnf_list y cnf_res
+Fixpoint min_element (l: list Z): Z :=
+  match l with
+    | nil => 0%Z
+    | h :: t => Z.min h (min_element t)
+  end.
+  
+Fixpoint max_cnf (l: cnf_list): Z :=
+  match l with
+    | nil => 0%Z
+    | clause :: t => Z.max (max_element clause) (max_cnf t)
+  end.
+
+Fixpoint min_cnf (l: cnf_list): Z :=
+  match l with
+    | nil => 0%Z
+    | clause :: t => Z.min (min_element clause) (min_cnf t)
+  end.
+
+Definition prop_cnt_inf (l: cnf_list): Z :=
+  Z.max (max_cnf l) (Z.abs (min_cnf l)).
+
+Definition store_predata (x: addr) (cnf_res: cnf_list) (prop_cnt clause_cnt: Z): Assertion :=
+ [| x <> NULL |] && [| Zlength cnf_res = clause_cnt |] &&
+ [| prop_cnt_inf cnf_res <= prop_cnt |] &&
+  EX y: addr,
+    &(x # "PreData" ->ₛ "cnf_res") # Ptr |-> y **
+    &(x # "PreData" ->ₛ "prop_cnt") # Int |-> prop_cnt **
+    &(x # "PreData" ->ₛ "clause_cnt") # Int |-> clause_cnt **
+    sll_cnf_list y cnf_res.
+
+(* Definition  (l: list Z): cnf_list_cell :=
+  CNFCell 3 l. *)
+
+Notation "x <>? y" := (negb (Z.eqb x y)) (at level 70).
+Notation "x ==? y" := (Z.eq_dec x y) (at level 70).
+
+Import smt_lang_enums1.
+
+(* p3 <-> (p1 op p2) to cnf *)
+Definition iff2cnf_binary (p1 p2 p3: Z) (op: SmtPropBop): cnf_list :=
+  match op with
+    | SMTPROP_AND => let c1 := [p1; -p3] in
+            let c2 := [p2; -p3] in
+              let c3 := if (p1 ==? p2) then [-p1; p3] else [-p1; -p2; p3] in
+                c1 :: c2 :: c3 :: nil
+    | SMTPROP_OR => let c1 := [-p1; p3] in
+            let c2 := [-p2; p3] in
+              let c3 := if (p1 ==? p2) then [p1; -p3] else [p1; p2; -p3] in
+                c1 :: c2 :: c3 :: nil
+    | SMTPROP_IMPLY => if (p1 ==? p2) then
+              ( (p3 :: nil)) :: nil
+           else
+            let c1 := [p1; p3] in
+              let c2 := [-p2; p3] in
+                let c3 := [-p1; p2; -p3] in
+                  c1 :: c2 :: c3 :: nil
+
+    | SMTPROP_IFF => if (p1 ==? p2) then
+            ( (p3 :: nil)) :: nil
+           else
+            let c1 := [p1; p2; p3] in
+              let c2 := [-p1; -p2; p3] in
+                let c3 := [p1; -p2; -p3] in
+                  let c4 := [-p1; p2; -p3] in
+                    c1 :: c2 :: c3 :: c4 :: nil
+  end.
+
+Definition iff2cnf_length_binary (p1 p2 p3: Z) (op: SmtPropBop): Z :=
+  match op with
+    | SMTPROP_AND => 3%Z
+    | SMTPROP_OR => 3%Z
+    | SMTPROP_IMPLY => if (p1 ==? p2) then 1%Z else 3%Z
+    | SMTPROP_IFF => if (p1 ==? p2) then 1%Z else 4%Z
+  end.
+
+Lemma iff2cnf_binary_and:
+  forall p1 p2 p3,
+    iff2cnf_binary p1 p2 p3 SMTPROP_AND =
+    [p1; -p3] :: [p2; -p3] :: (if (p1 ==? p2) then [-p1; p3] else [-p1; -p2; p3]) :: nil /\
+    iff2cnf_length_binary p1 p2 p3 SMTPROP_AND = 3%Z.
+Proof.
+  intros.
+  split; reflexivity.
+Qed.
+
+Lemma iff2cnf_binary_and_eq:
+  forall p1 p2 p3,
+    p1 = p2 ->
+    iff2cnf_binary p1 p2 p3 SMTPROP_AND =
+    [p1; -p3] :: [p2; -p3] :: [-p1; p3] :: nil /\
+    iff2cnf_length_binary p1 p2 p3 SMTPROP_AND = 3%Z.
+Proof.
+  intros.
+  unfold iff2cnf_binary, iff2cnf_length_binary.
+  split; destruct (p1 ==? p2); try reflexivity; try lia.
+Qed.
+
+Lemma iff2cnf_binary_and_neq:
+  forall p1 p2 p3,
+    p1 <> p2 ->
+    iff2cnf_binary p1 p2 p3 SMTPROP_AND =
+    [p1; -p3] :: [p2; -p3] :: [-p1; -p2; p3] :: nil /\
+    iff2cnf_length_binary p1 p2 p3 SMTPROP_AND = 3%Z.
+Proof.
+  intros.
+  unfold iff2cnf_binary, iff2cnf_length_binary.
+  split; destruct (p1 ==? p2); try reflexivity; try lia.
+Qed.
+
+Lemma iff2cnf_binary_or:
+  forall p1 p2 p3,
+    iff2cnf_binary p1 p2 p3 SMTPROP_OR =
+    [-p1; p3] :: [-p2; p3] :: (if (p1 ==? p2) then [p1; -p3] else [p1; p2; -p3]) :: nil /\
+    iff2cnf_length_binary p1 p2 p3 SMTPROP_OR = 3%Z.
+Proof.
+  intros.
+  split; reflexivity.
+Qed.
+
+Lemma iff2cnf_binary_or_eq:
+  forall p1 p2 p3,
+    p1 = p2 ->
+    iff2cnf_binary p1 p2 p3 SMTPROP_OR =
+    [-p1; p3] :: [-p2; p3] :: [p1; -p3] :: nil /\
+    iff2cnf_length_binary p1 p2 p3 SMTPROP_OR = 3%Z.
+Proof.
+  intros.
+  unfold iff2cnf_binary, iff2cnf_length_binary.
+  split; destruct (p1 ==? p2); try reflexivity; try lia.
+Qed.
+
+Lemma iff2cnf_binary_or_neq:
+  forall p1 p2 p3,
+    p1 <> p2 ->
+    iff2cnf_binary p1 p2 p3 SMTPROP_OR =
+    [-p1; p3] :: [-p2; p3] :: [p1; p2; -p3] :: nil /\
+    iff2cnf_length_binary p1 p2 p3 SMTPROP_OR = 3%Z.
+Proof.
+  intros.
+  unfold iff2cnf_binary, iff2cnf_length_binary.
+  split; destruct (p1 ==? p2); try reflexivity; try lia.
+Qed.
+
+Lemma iff2cnf_binary_imply_eq:
+  forall p1 p2 p3,
+    p1 = p2 ->
+    iff2cnf_binary p1 p2 p3 SMTPROP_IMPLY = [p3] :: nil /\
+    iff2cnf_length_binary p1 p2 p3 SMTPROP_IMPLY = 1%Z.
+Proof.
+  intros.
+  unfold iff2cnf_binary, iff2cnf_length_binary.
+  split; destruct (p1 ==? p2); try reflexivity; try lia.
+Qed.
+
+Lemma iff2cnf_binary_imply_neq:
+  forall p1 p2 p3,
+    p1 <> p2 ->
+    iff2cnf_binary p1 p2 p3 SMTPROP_IMPLY =
+    [p1; p3] :: [-p2; p3] :: [-p1; p2; -p3] :: nil /\
+    iff2cnf_length_binary p1 p2 p3 SMTPROP_IMPLY = 3%Z.
+Proof.
+  intros.
+  unfold iff2cnf_binary, iff2cnf_length_binary.
+  split; destruct (p1 ==? p2); try reflexivity; try lia.
+Qed.
+
+Lemma iff2cnf_binary_iff_eq:
+  forall p1 p2 p3,
+    p1 = p2 ->
+    iff2cnf_binary p1 p2 p3 SMTPROP_IFF = [p3] :: nil /\
+    iff2cnf_length_binary p1 p2 p3 SMTPROP_IFF = 1%Z.
+Proof.
+  intros.
+  unfold iff2cnf_binary, iff2cnf_length_binary.
+  split; destruct (p1 ==? p2); try reflexivity; try lia.
+Qed.
+
+Lemma iff2cnf_binary_iff_neq:
+  forall p1 p2 p3,
+    p1 <> p2 ->
+    iff2cnf_binary p1 p2 p3 SMTPROP_IFF =
+    [p1; p2; p3] :: [-p1; -p2; p3] :: [p1; -p2; -p3] :: [-p1; p2; -p3] :: nil /\
+    iff2cnf_length_binary p1 p2 p3 SMTPROP_IFF = 4%Z. 
+Proof.
+  intros.
+  unfold iff2cnf_binary, iff2cnf_length_binary.
+  split; destruct (p1 ==? p2); try reflexivity; try lia.
+Qed.
+
+Lemma iff2cnf_length_eq:
+  forall p1 p2 p3 op,
+    Zlength (iff2cnf_binary p1 p2 p3 op) = iff2cnf_length_binary p1 p2 p3 op.
+Proof.
+  intros.
+  unfold iff2cnf_binary, iff2cnf_length_binary, Zlength.
+  destruct op; simpl; try reflexivity.
+  + destruct (p1 ==? p2); simpl; try reflexivity; try lia.
+  + destruct (p1 ==? p2); simpl; try reflexivity; try lia.
+Qed.
+
+(* Definition iff2cnf_binary (p1 p2 p3: Z) (op: Z): cnf_list :=
+  match op with
+    | 0 => let c1 := [p1; -p3] in
+            let c2 := [p2; -p3] in
+              let c3 := if (p1 ==? p2) then [-p1; p3] else [-p1; -p2; p3] in
+                c1 :: c2 :: c3 :: nil
+    | 1 => let c1 := [-p1; p3] in
+            let c2 := [-p2; p3] in
+              let c3 := if (p1 ==? p2) then [p1; -p3] else [p1; p2; -p3] in
+                c1 :: c2 :: c3 :: nil
+    | 2 => if (p1 ==? p2) then
+              ( (p3 :: nil)) :: nil
+            else
+            let c1 := [p1; p3] in
+              let c2 := [-p2; p3] in
+                let c3 := [-p1; p2; -p3] in
+                  c1 :: c2 :: c3 :: nil
+
+    | 3 => if (p1 ==? p2) then
+            ( (p3 :: nil)) :: nil
+            else
+            let c1 := [p1; p2; p3] in
+              let c2 := [-p1; -p2; p3] in
+                let c3 := [p1; -p2; -p3] in
+                  let c4 := [-p1; p2; -p3] in
+                    c1 :: c2 :: c3 :: c4 :: nil
+    | _ => nil
+  end.
+
+Definition iff2cnf_length_binary (p1 p2 p3: Z) (op: Z): Z :=
+  match op with
+    | 0 => 3%Z
+    | 1 => 3%Z
+    | 2 => if (p1 ==? p2) then 1%Z else 3%Z
+    | 3 => if (p1 ==? p2) then 1%Z else 4%Z
+    | _ => 0%Z
+  end. *)
+
+Definition iff2cnf_unary (p2 p3: Z): cnf_list :=
+  let c1 := [p2; p3] in
+    let c2 := [-p2; -p3] in
+      c1 :: c2 :: nil.
+
+  (* 0 => AND
+     1 => OR
+     2 => IMPLY
+     3 => IFF
+     4 => NOT *)
+
+Fixpoint max_var_SmtProp (s: smt_prop): Z :=
+  match s with
+    | SmtB op lt rt => Z.max (max_var_SmtProp lt) (max_var_SmtProp rt)
+    | SmtU op prop => max_var_SmtProp prop
+    | SmtV var => var
+  end.
+
+Fixpoint min_var_SmtProp (s: smt_prop): Z :=
+  match s with
+    | SmtB op lt rt => Z.min (min_var_SmtProp lt) (min_var_SmtProp rt)
+    | SmtU op prop => min_var_SmtProp prop
+    | SmtV var => var
+  end.
+
+Definition prop_cnt_inf_SmtProp (s: smt_prop): Z :=
+  Z.max (max_var_SmtProp s) (Z.abs (min_var_SmtProp s)).
+
+Definition PreData : Type := cnf_list * Z * Z.
+Definition prop2cnf_ret : Type := PreData * Z.
+
+Definition make_predata (cnf_res: cnf_list) (prop_cnt clause_cnt: Z): PreData :=
+  (cnf_res, prop_cnt, clause_cnt).
+
+Definition make_prop2cnf_ret (data: PreData) (ret: Z): prop2cnf_ret :=
+  (data, ret).
+
+Fixpoint prop2cnf_logic (s: smt_prop) (data: PreData): prop2cnf_ret :=
+  match s with
+    | SmtB op lt rt =>
+      let (data1, p1) := prop2cnf_logic lt data in
+      let (data2, p2) := prop2cnf_logic rt data1 in
+      let (tmp, clause_cnt) := data2 in
+      let (cnf_res, prop_cnt) := tmp in
+      let cnf_gen := (iff2cnf_binary p1 p2 (prop_cnt + 1) op) in
+      let len_gen := (iff2cnf_length_binary p1 p2 (prop_cnt + 1) op) in
+      let data_ret := ((app cnf_gen cnf_res), (prop_cnt + 1), (clause_cnt + len_gen)) in
+      (data_ret, prop_cnt + 1)
+
+    | SmtU op prop =>
+      let (data1, p1) := prop2cnf_logic prop data in
+      let (tmp, clause_cnt) := data1 in
+      let (cnf_res, prop_cnt) := tmp in
+      let cnf_gen := (iff2cnf_unary p1 (prop_cnt + 1)) in
+      let data_ret := ((app cnf_gen cnf_res), (prop_cnt + 1), (clause_cnt + 2)) in
+      (data_ret, prop_cnt + 1)
+
+    | SmtV var => (data, var)
   end.
