qcp/cnf/VC/cnf_trans_proof_manual.v
@@ -1,0 +1,208 @@
+Require Import Coq.ZArith.ZArith.
+Require Import Coq.Bool.Bool.
+Require Import Coq.Strings.String.
+Require Import Coq.Lists.List.
+Require Import Coq.Classes.RelationClasses.
+Require Import Coq.Classes.Morphisms.
+Require Import Coq.micromega.Psatz.
+Require Import Coq.Sorting.Permutation.
+From AUXLib Require Import int_auto Axioms Feq Idents List_lemma VMap.
+Require Import SetsClass.SetsClass. Import SetsNotation.
+From SimpleC.SL Require Import Mem SeparationLogic.
+Require Import cnf_trans_goal.
+Require Import Logic.LogicGenerator.demo932.Interface.
+Local Open Scope Z_scope.
+Local Open Scope sets.
+Local Open Scope string.
+Local Open Scope list.
+Import naive_C_Rules.
+Import naive_C_Rules.
+Require Import smt_lang_lib.
+Require Import cnf_trans_lib.
+From SimpleC.EE Require Import malloc.
+From SimpleC.EE Require Import sll_tmpl.
+Local Open Scope sac.
+
+Lemma proof_of_clause_gen_unary_safety_wit_5 : clause_gen_unary_safety_wit_5.
+Proof.  
+
+Lemma proof_of_clause_gen_unary_safety_wit_7 : clause_gen_unary_safety_wit_7.
+Proof. Admitted. 
+
+Lemma proof_of_clause_gen_unary_safety_wit_8 : clause_gen_unary_safety_wit_8.
+Proof. Admitted. 
+
+Lemma proof_of_clause_gen_unary_return_wit_1 : clause_gen_unary_return_wit_1.
+Proof. Admitted. 
+
+Lemma proof_of_clause_gen_unary_which_implies_wit_1 : clause_gen_unary_which_implies_wit_1.
+Proof. Admitted. 
+
+Lemma proof_of_clause_gen_binary_safety_wit_5 : clause_gen_binary_safety_wit_5.
+Proof. Admitted. 
+
+Lemma proof_of_clause_gen_binary_safety_wit_8 : clause_gen_binary_safety_wit_8.
+Proof. Admitted. 
+
+Lemma proof_of_clause_gen_binary_safety_wit_13 : clause_gen_binary_safety_wit_13.
+Proof. Admitted. 
+
+Lemma proof_of_clause_gen_binary_safety_wit_16 : clause_gen_binary_safety_wit_16.
+Proof. Admitted. 
+
+Lemma proof_of_clause_gen_binary_safety_wit_24 : clause_gen_binary_safety_wit_24.
+Proof. Admitted. 
+
+Lemma proof_of_clause_gen_binary_safety_wit_27 : clause_gen_binary_safety_wit_27.
+Proof. Admitted. 
+
+Lemma proof_of_clause_gen_binary_safety_wit_29 : clause_gen_binary_safety_wit_29.
+Proof. Admitted. 
+
+Lemma proof_of_clause_gen_binary_safety_wit_31 : clause_gen_binary_safety_wit_31.
+Proof. Admitted. 
+
+Lemma proof_of_clause_gen_binary_safety_wit_34 : clause_gen_binary_safety_wit_34.
+Proof. Admitted. 
+
+Lemma proof_of_clause_gen_binary_safety_wit_44 : clause_gen_binary_safety_wit_44.
+Proof. Admitted. 
+
+Lemma proof_of_clause_gen_binary_safety_wit_47 : clause_gen_binary_safety_wit_47.
+Proof. Admitted. 
+
+Lemma proof_of_clause_gen_binary_safety_wit_50 : clause_gen_binary_safety_wit_50.
+Proof. Admitted. 
+
+Lemma proof_of_clause_gen_binary_safety_wit_61 : clause_gen_binary_safety_wit_61.
+Proof. Admitted. 
+
+Lemma proof_of_clause_gen_binary_safety_wit_63 : clause_gen_binary_safety_wit_63.
+Proof. Admitted. 
+
+Lemma proof_of_clause_gen_binary_safety_wit_67 : clause_gen_binary_safety_wit_67.
+Proof. Admitted. 
+
+Lemma proof_of_clause_gen_binary_safety_wit_69 : clause_gen_binary_safety_wit_69.
+Proof. Admitted. 
+
+Lemma proof_of_clause_gen_binary_safety_wit_71 : clause_gen_binary_safety_wit_71.
+Proof. Admitted. 
+
+Lemma proof_of_clause_gen_binary_safety_wit_74 : clause_gen_binary_safety_wit_74.
+Proof. Admitted. 
+
+Lemma proof_of_clause_gen_binary_safety_wit_98 : clause_gen_binary_safety_wit_98.
+Proof. Admitted. 
+
+Lemma proof_of_clause_gen_binary_safety_wit_100 : clause_gen_binary_safety_wit_100.
+Proof. Admitted. 
+
+Lemma proof_of_clause_gen_binary_safety_wit_130 : clause_gen_binary_safety_wit_130.
+Proof. Admitted. 
+
+Lemma proof_of_clause_gen_binary_safety_wit_132 : clause_gen_binary_safety_wit_132.
+Proof. Admitted. 
+
+Lemma proof_of_clause_gen_binary_safety_wit_134 : clause_gen_binary_safety_wit_134.
+Proof. Admitted. 
+
+Lemma proof_of_clause_gen_binary_safety_wit_136 : clause_gen_binary_safety_wit_136.
+Proof. Admitted. 
+
+Lemma proof_of_clause_gen_binary_safety_wit_138 : clause_gen_binary_safety_wit_138.
+Proof. Admitted. 
+
+Lemma proof_of_clause_gen_binary_safety_wit_140 : clause_gen_binary_safety_wit_140.
+Proof. Admitted. 
+
+Lemma proof_of_clause_gen_binary_safety_wit_142 : clause_gen_binary_safety_wit_142.
+Proof. Admitted. 
+
+Lemma proof_of_clause_gen_binary_return_wit_1_1 : clause_gen_binary_return_wit_1_1.
+Proof. Admitted. 
+
+Lemma proof_of_clause_gen_binary_return_wit_1_2 : clause_gen_binary_return_wit_1_2.
+Proof. Admitted. 
+
+Lemma proof_of_clause_gen_binary_return_wit_1_3 : clause_gen_binary_return_wit_1_3.
+Proof. Admitted. 
+
+Lemma proof_of_clause_gen_binary_return_wit_1_4 : clause_gen_binary_return_wit_1_4.
+Proof. Admitted. 
+
+Lemma proof_of_clause_gen_binary_return_wit_1_5 : clause_gen_binary_return_wit_1_5.
+Proof. Admitted. 
+
+Lemma proof_of_clause_gen_binary_return_wit_1_6 : clause_gen_binary_return_wit_1_6.
+Proof. Admitted. 
+
+Lemma proof_of_clause_gen_binary_return_wit_1_7 : clause_gen_binary_return_wit_1_7.
+Proof. Admitted. 
+
+Lemma proof_of_clause_gen_binary_return_wit_1_8 : clause_gen_binary_return_wit_1_8.
+Proof. Admitted. 
+
+Lemma proof_of_clause_gen_binary_return_wit_1_9 : clause_gen_binary_return_wit_1_9.
+Proof. Admitted. 
+
+Lemma proof_of_clause_gen_binary_which_implies_wit_1 : clause_gen_binary_which_implies_wit_1.
+Proof. Admitted. 
+
+Lemma proof_of_prop2cnf_safety_wit_3 : prop2cnf_safety_wit_3.
+Proof. Admitted. 
+
+Lemma proof_of_prop2cnf_safety_wit_6 : prop2cnf_safety_wit_6.
+Proof. Admitted. 
+
+Lemma proof_of_prop2cnf_safety_wit_9 : prop2cnf_safety_wit_9.
+Proof. Admitted. 
+
+Lemma proof_of_prop2cnf_entail_wit_1 : prop2cnf_entail_wit_1.
+Proof. Admitted. 
+
+Lemma proof_of_prop2cnf_entail_wit_2 : prop2cnf_entail_wit_2.
+Proof. Admitted. 
+
+Lemma proof_of_prop2cnf_return_wit_1_1 : prop2cnf_return_wit_1_1.
+Proof. Admitted. 
+
+Lemma proof_of_prop2cnf_return_wit_1_2 : prop2cnf_return_wit_1_2.
+Proof. Admitted. 
+
+Lemma proof_of_prop2cnf_return_wit_1_3 : prop2cnf_return_wit_1_3.
+Proof. Admitted. 
+
+Lemma proof_of_prop2cnf_partial_solve_wit_5_pure : prop2cnf_partial_solve_wit_5_pure.
+Proof. Admitted. 
+
+Lemma proof_of_prop2cnf_which_implies_wit_1 : prop2cnf_which_implies_wit_1.
+Proof. Admitted. 
+
+Lemma proof_of_prop2cnf_which_implies_wit_2 : prop2cnf_which_implies_wit_2.
+Proof. Admitted. 
+
+Lemma proof_of_prop2cnf_which_implies_wit_3 : prop2cnf_which_implies_wit_3.
+Proof. Admitted. 
+
+Lemma proof_of_prop2cnf_which_implies_wit_4 : prop2cnf_which_implies_wit_4.
+Proof. Admitted. 
+
+Lemma proof_of_prop2cnf_which_implies_wit_6 : prop2cnf_which_implies_wit_6.
+Proof. Admitted. 
+
+Lemma proof_of_prop2cnf_which_implies_wit_8 : prop2cnf_which_implies_wit_8.
+Proof. Admitted. 
+
+Lemma proof_of_prop2cnf_which_implies_wit_9 : prop2cnf_which_implies_wit_9.
+Proof. Admitted. 
+
+Lemma proof_of_prop2cnf_which_implies_wit_10 : prop2cnf_which_implies_wit_10.
+Proof. Admitted. 
+
+Lemma proof_of_prop2cnf_which_implies_wit_12 : prop2cnf_which_implies_wit_12.
+Proof. Admitted. 
+
+Lemma proof_of_prop2cnf_which_implies_wit_14 : prop2cnf_which_implies_wit_14.
+Proof. Admitted. 
+
